TickGenerator.v
@@ -1,0 +1,64 @@
+(** * A box to prevent timing side channels (part of TCB) *)
+Require Import Coq.Program.Basics Coq.NArith.NArith Coq.Lists.List.
+Require Import FunctionApp TrustedTickBox.
+
+Set Implicit Arguments.
+
+Local Open Scope list_scope.
+Local Open Scope program_scope.
+
+Section tickG.
+
+  Context (world : Type).
+
+  Inductive tickGInput :=
+  | TGWakeUp
+  | TGClocksGot (nanoseconds : N).
+
+  Definition nanos_per_tick := 1%N.
+  Definition sleep_nanos := 1024%N.
+
+  Open Scope N_scope.
+
+  Inductive tickGOutput :=
+  | TGSleepNanosecs (_ : N)
+  | TGGetNanosecs
+  | TGTick (_ : N).
+
+  Definition GatewayState := option N.
+
+  Definition tickGLoopPreBody (st : option N) : tickGInput -> (list tickGOutput) * GatewayState :=
+    fun i =>
+      match i with
+        | TGWakeUp =>
+          (TGGetNanosecs :: nil, st)
+        | TGClocksGot new =>
+          let actions :=
+              match st with
+                | Some prev => 
+                  let ticks := (new - prev) / nanos_per_tick in
+                  TGTick ticks :: nil
+                | None => nil
+              end in
+          (TGSleepNanosecs sleep_nanos :: actions, Some new)
+      end.
+
+  Context (handle : tickGOutput -> action world).
+
+  Definition tickGLoopBody {T}
+             (loop : GatewayState -> T)
+             (st : GatewayState)
+  : tickGInput -> action world * T
+    := fun i => let outputs := fst (tickGLoopPreBody st i) in
+                let st' := snd (tickGLoopPreBody st i) in
+                (fold_left compose (map handle outputs) id,
+                 loop st').
+
+  CoFixpoint tickGLoop (st : option N) :=
+    Step (tickGLoopBody tickGLoop st).
+
+  Definition tickGInitState : GatewayState := None.
+
+  Definition tickG := tickGLoop tickGInitState.
+
+End tickG.
