TrustedServerSyncBox.v
@@ -1,6 +1,6 @@
 (** * A box to mirror a server over untrusted channels using encryption while preventing timing side channels (part of TCB) *)
 Require Import Coq.Program.Basics Coq.NArith.NArith Coq.Lists.List.
-Require Import FunctionApp EncryptionInterface TrustedTickBox TrustedTickBoxWrapper TrustedEncryptBox TrustedDecryptBox.
+Require Import FunctionApp EncryptionInterface TrustedTickBox TrustedEncryptBox TrustedDecryptBox.
 Require Import Common.
 
 Local Open Scope list_scope.
@@ -138,8 +138,7 @@ for field0, ty0 in fields:
     | ssbClientSet (newD : rawDataT)
     | ssbServerGotUpdate (newE : encryptedDataT)
     | ssbSystemRandomness (randomness : systemRandomnessT) (tag : rawDataT)
-    | ssbWakeUp
-    | ssbClocksGot (_ : N).
+    | ssbTick (_ : N).
 
     Definition ssbInput := (ssbConfigInput + ssbEventInput)%type.
 
@@ -155,9 +154,7 @@ for field0, ty0 in fields:
     | ssbClientGotUpdate (data : rawDataT)
     | ssbServerGetUpdate
     | ssbServerCAS (curE newE : encryptedDataT)
-    | ssbRequestSystemRandomness (howMuch : systemRandomnessHintT) (tag : rawDataT)
-    | ssbSleepNanosecs (nanos : N)
-    | ssbGetNanosecs.
+    | ssbRequestSystemRandomness (howMuch : systemRandomnessHintT) (tag : rawDataT).
 
     Definition ssbOutput := (ssbWarningOutput + ssbEventOutput)%type.
 
@@ -169,8 +166,8 @@ for field0, ty0 in fields:
       {|
         ssbState := {| localStateD := initRawData;
                        remoteStateE := None |};
-        ssbGetUpdateState := TrustedTickBoxWrapper.initState _;
-        ssbCASState := TrustedTickBoxWrapper.initState _;
+        ssbGetUpdateState := TrustedTickBox.initState _;
+        ssbCASState := TrustedTickBox.initState _;
         ssbEncryptState := TEB.initState;
         ssbDecryptState := TDB.initState
       |}.
@@ -227,10 +224,6 @@ for field0, ty0 in fields:
                         end eq_refl
                    | inr (tbPublishUpdate val)
                      => inr ssbServerGetUpdate::nil
-                   | inr (tbSleepNanosecs n)
-                     => inr (ssbSleepNanosecs n) :: nil
-                   | inr tbGetNanosecs
-                     => inr ssbGetNanosecs :: nil
                  end,
                  set_ssbGetUpdateState st (snd i)));
       handle_eq_false.
@@ -306,10 +299,6 @@ for field0, ty0 in fields:
                                           (st'.(ssbEncryptState))
                                           (ebEncrypt (st.(localStateD)) tt) in
                        handle_ssbEncrypt st' encResult
-                  | inr (tbSleepNanosecs n)
-                    => (inr (ssbSleepNanosecs n) :: nil, st')
-                  | inr tbGetNanosecs
-                    => (inr ssbGetNanosecs :: nil, st')
                 end).
     Defined.
 
@@ -373,30 +362,17 @@ for field0, ty0 in fields:
                                               (dbSetMasterKey _ newKey)) in
                        (ls0 ++ ls1, st1)
 
-                  | inr ssbWakeUp
+                  | inr (ssbTick n)
                     => let (ls0, st0) := handle_ssbGetUpdate
                                            st
                                            (tickBoxLoopPreBody
                                               (st.(ssbGetUpdateState))
-                                              (inr (tbWakeUp _))) in
+                                              (inr (tbTick _ n))) in
                        let (ls1, st1) := handle_ssbCAS
                                            st0
                                            (tickBoxLoopPreBody
                                               (st0.(ssbCASState))
-                                              (inr (tbWakeUp _))) in
-                       (ls0 ++ ls1, st1)
-
-                  | inr (ssbClocksGot n)
-                    => let (ls0, st0) := handle_ssbGetUpdate
-                                           st
-                                           (tickBoxLoopPreBody
-                                              (st.(ssbGetUpdateState))
-                                              (inr (tbClocksGot _ n))) in
-                       let (ls1, st1) := handle_ssbCAS
-                                           st0
-                                           (tickBoxLoopPreBody
-                                              (st0.(ssbCASState))
-                                              (inr (tbClocksGot _ n))) in
+                                              (inr (tbTick _ n))) in
                        (ls0 ++ ls1, st1)
 
                   | inr ssbClientGetUpdate
